refactoring extraction, sized types, etc

GPU.h
@@ -1,6 +1,39 @@
 #ifndef __PULSE__GPU_H
 #define __PULSE__GPU_H 1
 
+#include <assert.h>
+#include <stdint.h>
+
 #define PULSE_KCALL(foo, nblk, nthr, ...) foo<<<nblk,nthr>>>(__VA_ARGS__)
+
+static inline
+uint32_t * PULSE_GPU_ALLOC(size_t len)
+{
+	uint32_t *ret = NULL;
+	if (cudaMalloc(&ret, len) != cudaSuccess)
+		assert(0);
+	return ret;
+}
+
+static inline
+void PULSE_GPU_FREE(void *p)
+{
+	if (cudaFree(p) != cudaSuccess)
+		assert(0);
+}
+
+static inline
+void PULSE_GPU_MEMCPY_H2D(void *p, void *gp, size_t sz)
+{
+	if (cudaMemcpy(gp, p, sz, cudaMemcpyHostToDevice) != cudaSuccess)
+		assert(0);
+}
+
+static inline
+void PULSE_GPU_MEMCPY_D2H(void *p, void *gp, size_t sz)
+{
+	if (cudaMemcpy(p, gp, sz, cudaMemcpyDeviceToHost) != cudaSuccess)
+		assert(0);
+}
 
 #endif
