src/examples/GPU.DotProduct.fst
@@ -101,8 +101,8 @@ fn main (_:unit)
   let ga1 = gpu_array_alloc #U32.t m_size;
   let ga2 = gpu_array_alloc #U32.t m_size;
 
-  GPU.Array.gpu_memcpy_host_to_device a1 ga1;
-  GPU.Array.gpu_memcpy_host_to_device a2 ga2;
+  GPU.Array.gpu_memcpy_host_to_device a1 ga1 m_size;
+  GPU.Array.gpu_memcpy_host_to_device a2 ga2 m_size;
   
   let gr = gpu_array_alloc #U32.t m_size;
   
@@ -157,7 +157,7 @@ fn main (_:unit)
   (**)gpu_array_unslice_1_underspec ga2;
   (**)gpu_array_unslice_1_underspec gr;
   
-  GPU.Array.gpu_memcpy_device_to_host ar gr;
+  GPU.Array.gpu_memcpy_device_to_host ar gr m_size;
   gpu_array_free ga1;
   gpu_array_free ga2;
   gpu_array_free gr;
