src/lib/GPU.fsti
@@ -2,6 +2,7 @@ module GPU
 
 include GPU.Base
 include GPU.Ref
+include GPU.Types
 include GPU.Array
 include GPU.SizeT
 include GPU.Barrier2
